Loops_float.v
@@ -382,7 +382,7 @@ Tactic Notation "xfor_sum_fma" constr(Inv) constr(R) uconstr(R') uconstr(op) con
   eapply (@xfor_big_op_lemma_extended _ _ _ _ Inv R R' val_float float_unit (float_unit, float_unit) (fun a (b : binary64 * binary64) => @BFMA _ Tdouble b.1 b.2 a) 
     (fun (b : binary64 * binary64) => @finite Tdouble b.1 /\ @finite Tdouble b.2) op s);
   [ let L := fresh in 
-    intros ?? L;
+    intros ?? L; rewrite ?/Inv ?/R ?/R';
     xnsimpl
   | disjointE
   | xfor_sum_cong_solve op
