Unary_IndexWithBounds.v
@@ -35,10 +35,6 @@ Proof Build_Inhab (ex_intro (fun=> True) (Lab (0, 0) 0) I). *)
       k++
 *)
 
-Global Instance Inhab_lab_int : Inhab (labeled int).
-split. by exists (Lab (0,0) 0). Qed.
-
-
 Module and.
 Section and.
 
